Hoare if1

softwarefoundations/vol2_plf/Hoare.v
@@ -6,3 +6,502 @@ From Coq Require Import Arith.EqNat.
 From Coq Require Import Arith.PeanoNat. Import Nat.
 From Coq Require Import Lia.
 From PLF Require Export Imp.
+
+From Coq Require Import Logic.FunctionalExtensionality.
+
+Definition Assertion := state -> Prop.
+
+Module ExAssertions.
+  Definition assn1 : Assertion := fun st => st X <= st Y.
+  Definition assn2 : Assertion := fun st => st X = 3 \/ st X <= st Y.
+  Definition assn3 : Assertion := fun st => st Z * st Z <= st X /\ ~ (((S (st Z)) * (S (st Z))) <= st X).
+  Definition assn4 : Assertion := fun st => st Z = max (st X) (st Y).
+End ExAssertions.
+
+Definition assert_implies (P Q : Assertion) : Prop := forall st, P st -> Q st.
+
+Declare Scope hoare_spec_scope.
+Notation "P ->> Q" := (assert_implies P Q)
+                      (at level 80) : hoare_spec_scope.
+Open Scope hoare_spec_scope.
+Notation "P <<->> Q" := (P ->> Q /\ Q ->> P) 
+                        (at level 80) : hoare_spec_scope.
+
+Definition Aexp : Type := state -> nat.
+Definition assert_of_Prop (P : Prop) : Assertion := fun _ => P.
+Definition Aexp_of_nat (n : nat) : Aexp := fun _ => n.
+Definition Aexp_of_aexp (a : aexp) : Aexp := fun st => aeval st a.
+
+Coercion assert_of_Prop : Sortclass >-> Assertion.
+Coercion Aexp_of_nat : nat >-> Aexp.
+Coercion Aexp_of_aexp : aexp >-> Aexp.
+
+Arguments assert_of_Prop /.
+Arguments Aexp_of_nat /.
+Arguments Aexp_of_aexp /.
+
+Declare Scope assertion_scope.
+Bind Scope assertion_scope with Assertion.
+Bind Scope assertion_scope with Aexp.
+Delimit Scope assertion_scope with assertion.
+Notation assert P := (P%assertion : Assertion).
+Notation mkAexp a := (a%assertion : Aexp).
+Notation "~ P"      := (fun st => ~ assert P st) : assertion_scope.
+Notation "P /\ Q"   := (fun st => assert P st /\ assert Q st) : assertion_scope.
+Notation "P \/ Q"   := (fun st => assert P st \/ assert Q st) : assertion_scope.
+Notation "P -> Q"   := (fun st => assert P st -> assert Q st) : assertion_scope.
+Notation "P <-> Q"  := (fun st => assert P st <-> assert Q st) : assertion_scope.
+Notation "a = b"    := (fun st => mkAexp a st = mkAexp b st) : assertion_scope.
+Notation "a <> b"   := (fun st => mkAexp a st <> mkAexp b st) : assertion_scope.
+Notation "a <= b"   := (fun st => mkAexp a st <= mkAexp b st) : assertion_scope.
+Notation "a < b"    := (fun st => mkAexp a st < mkAexp b st) : assertion_scope.
+Notation "a >= b"   := (fun st => mkAexp a st >= mkAexp b st) : assertion_scope.
+Notation "a > b"    := (fun st => mkAexp a st > mkAexp b st) : assertion_scope.
+Notation "a + b"    := (fun st => mkAexp a st + mkAexp b st) : assertion_scope.
+Notation "a - b"    := (fun st => mkAexp a st - mkAexp b st) : assertion_scope.
+Notation "a * b"    := (fun st => mkAexp a st * mkAexp b st) : assertion_scope.
+
+Definition ap {X} (f : nat -> X) (x : Aexp) := fun st => f (x st).
+Definition ap2 {X} (f : nat -> nat -> X) (x : Aexp) (y : Aexp) (st : state) := f (x st) (y st).
+
+Module ExPrettyAssertions.
+  Definition ex1 : Assertion := X = 3.
+  Definition ex2 : Assertion := True.
+  Definition ex3 : Assertion := False.
+  Definition assn1 : Assertion := X <= Y.
+  Definition assn2 : Assertion := X = 3 \/ X <= Y.
+  Definition assn3 : Assertion := Z * Z <= X /\ ~ (((ap S Z) * (ap S Z)) <= X).
+  Definition assn4 : Assertion := Z = ap2 max X Y.
+End ExPrettyAssertions.
+
+
+Definition hoare_triple (P : Assertion) (c : com) (Q : Assertion) : Prop :=
+  forall st st', st =[ c ]=> st' -> P st -> Q st'.
+
+Notation "{{ P }} c {{ Q }}" :=
+  (hoare_triple P c Q) (at level 90, c custom com at level 99)
+  : hoare_spec_scope.
+
+Check ({{True}} X := 0 {{True}}).
+
+
+Theorem hoare_post_true : forall (P Q : Assertion) c,
+  (forall st, Q st) -> {{P}} c {{Q}}.
+Proof.
+  intros P Q c H.
+  unfold hoare_triple.
+  intros st st' cmd Hp.
+  apply  (H st').
+Qed.
+
+Theorem hoare_pre_false : forall (P Q : Assertion) c,
+  (forall st, ~ (P st)) -> {{P}} c {{Q}}.
+Proof.
+  intros P Q c H. unfold hoare_triple. intros st st' cmd Hp.
+  exfalso.
+  apply (H st).
+  assumption.
+Qed.
+
+
+
+Definition assn_sub X a (P:Assertion) : Assertion :=
+  fun (st : state) => P (X !-> aeval st a ; st).
+
+Notation "P [ X |-> a ]" := (assn_sub X a P)
+                           (at level 10, X at next level, a custom com).
+
+Theorem hoare_asgn : forall Q X a,
+  {{Q [X |-> a]}} (X := a) {{Q}}.
+Proof. intros Q X a. unfold hoare_triple. intros st st' cmd Hq.
+  inversion cmd. subst.
+  unfold assn_sub in Hq. apply Hq. Qed.
+
+Example assn_sub_example :
+  {{(X < 5) [X |-> X + 1]}} X := X + 1 {{X < 5}}.
+Proof.
+  apply hoare_asgn. Qed.
+
+Example hoare_asgn_examples1 :
+  exists P, {{ P }} X := 2 * X {{ X <= 10 }}.
+Proof.
+  exists (assert (X <= 5)).
+  unfold hoare_triple. intros st st' cmd Hq.
+  simpl in *.
+  inversion cmd. subst. unfold t_update.
+  simpl. lia.
+Qed.
+
+Example hoare_asgn_examples2 :
+  exists P, {{ P }} X := 3 {{ 0 <= X /\ X <= 5 }}.
+Proof.
+  exists True.
+  unfold hoare_triple. intros st st' cmd Hq.
+  simpl.
+  inversion cmd; subst; simpl in *.
+  unfold t_update; simpl. lia.
+Qed.
+
+Example vice_versa_wrong: 
+  exists a, ~ ({{ True }} X := a {{ X = a }}).
+Proof.
+  exists (<{ X + 1 }>).
+  unfold hoare_triple.
+  intros H. simpl in H.
+  assert (G: 1 = 1 + 1). {
+    apply (H (X !-> 0) (X !-> 1; X !-> 0)).
+    apply E_Asgn. simpl.
+    reflexivity.
+    apply I.
+  }
+  discriminate G.
+Qed.
+
+Lemma qwe: forall st X (n: nat),
+  (X !-> st X; X !-> n; st) = st.
+Proof.
+  intros st X n.
+  unfold t_update. unfold eqb_string.
+  apply functional_extensionality.
+  intros x.
+  destruct (string_dec X x) as [E | E].
+  - rewrite E. reflexivity.
+  - reflexivity.
+Qed.
+
+Theorem hoare_asgn_fwd : forall m a P,
+  {{fun st => P st /\ st X = m}}
+    X := a
+  {{fun st => P (X !-> m ; st) /\ st X = aeval (X !-> m ; st) a }}.
+Proof.
+  unfold hoare_triple.
+  intros m a P st st' comm [Hpst Estx].
+  inversion comm; subst.
+  rewrite qwe. unfold t_update; simpl.
+  split.
+  - assumption.
+  - reflexivity.
+Qed.
+
+Lemma asd: forall X a st st',
+  st =[ X := a ]=> st' -> exists m, (X !-> m; st') = st.
+Proof.
+  intros X a st st' H.
+  inversion H; subst; simpl in *.
+  exists (st X).
+  apply qwe.
+Qed.
+
+
+Theorem hoare_asgn_fwd_exists : forall a P,
+  {{fun st => P st}}
+    X := a
+  {{fun st => exists m, P (X !-> m ; st) /\ st X = aeval (X !-> m ; st) a }}.
+Proof.
+  unfold hoare_triple.
+  intros a P st st' comm Hp.
+  inversion comm; subst; simpl in *.
+  destruct (asd _ _ _ _ comm) as [m' Hst].
+  exists m'.
+  rewrite Hst.
+  unfold t_update; simpl.
+  split.
+  - assumption.
+  - reflexivity.
+Qed.
+
+
+
+Theorem hoare_consequence_pre : forall (P P' Q : Assertion) c,
+  {{P'}} c {{Q}} ->  P ->> P'  -> {{P}} c {{Q}}.
+Proof. intros P P' Q c H1 H2.
+  unfold hoare_triple in *.
+  intros st st' c' Hpst.
+  apply (H1 st st' c' (H2 st Hpst)).
+Qed.
+
+Theorem hoare_consequence_post : forall (P Q Q' : Assertion) c,
+  {{P}} c {{Q'}} ->  Q' ->> Q  -> {{P}} c {{Q}}.
+Proof.
+  intros P Q Q' c H1 H2.
+  unfold hoare_triple in *.
+  intros st st' c' Hpst.
+  apply H2.
+  apply (H1 st st' c' Hpst).
+Qed.
+
+
+Example hoare_asgn_example1 :
+  {{True}} X := 1 {{X = 1}}.
+Proof.
+  (* WORKED IN CLASS *)
+  apply hoare_consequence_pre with (P' := (X = 1) [X |-> 1]).
+  - apply hoare_asgn.
+  - unfold "->>", assn_sub, t_update.
+    intros st _. simpl. reflexivity.
+Qed.
+
+Example assn_sub_example2 :
+  {{X < 4}} X := X + 1 {{X < 5}}.
+Proof.
+  (* WORKED IN CLASS *)
+  apply hoare_consequence_pre with (P' := (X < 5) [X |-> X + 1]).
+  - apply hoare_asgn.
+  - unfold "->>", assn_sub, t_update.
+    intros st H. simpl in *. lia.
+Qed.
+
+
+Theorem hoare_consequence : forall (P P' Q Q' : Assertion) c,
+  {{P'}} c {{Q'}} ->  P ->> P' -> Q' ->> Q ->  {{P}} c {{Q}}.
+Proof. intros.
+  apply (hoare_consequence_pre) with (P' := P').
+    - apply (hoare_consequence_post) with (Q' := Q').
+      + apply H.
+      + apply H1.
+    - apply H0.
+Qed.
+
+
+(* Hints for auto tactic *)
+Hint Unfold assert_implies hoare_triple assn_sub t_update : core.
+Hint Unfold assert_of_Prop Aexp_of_nat Aexp_of_aexp : core.
+
+Theorem hoare_consequence_pre''' : forall (P P' Q : Assertion) c,
+  {{P'}} c {{Q}} ->   P ->> P' ->  {{P}} c {{Q}}.
+Proof.
+  unfold hoare_triple, "->>".
+  intros P P' Q c Hhoare Himp st st' Heval Hpre.
+  eapply Hhoare.
+  - eassumption.
+  - apply Himp. assumption.
+Qed.
+
+
+Theorem hoare_consequence_pre'''' : forall (P P' Q : Assertion) c,
+  {{P'}} c {{Q}} ->   P ->> P' ->  {{P}} c {{Q}}.
+Proof. eauto. Qed.
+
+
+Ltac assn_auto :=
+  try auto; (* as in example 1, above *)
+  try (unfold "->>", assn_sub, t_update;
+       intros; simpl in *; lia). (* as in example 2 *)
+
+Example assn_sub_ex1' :
+  {{ X <= 5 }}  X := 2 * X  {{ X <= 10 }}.
+Proof.
+  eapply hoare_consequence_pre.
+  - apply hoare_asgn.
+  - assn_auto.
+Qed.
+
+Example assn_sub_ex2' :
+  {{ 0 <= 3 /\ 3 <= 5 }}  X := 3  {{ 0 <= X /\ X <= 5 }}.
+Proof.
+  eapply hoare_consequence_pre.
+  - apply hoare_asgn.
+  - assn_auto.
+Qed.
+
+
+
+
+Theorem hoare_skip : forall P,
+     {{P}} skip {{P}}.
+Proof. unfold hoare_triple. intros P st st' Hcomm Hpst.
+  inversion Hcomm; subst. assumption.
+Qed.
+
+
+Theorem hoare_seq : forall P Q R c1 c2,
+     {{Q}} c2 {{R}} -> {{P}} c1 {{Q}} -> {{P}} c1; c2 {{R}}.
+Proof. intros P Q R c1 c2 H1 H2. unfold hoare_triple in *. intros st st' Hcomm Hpst.
+  inversion Hcomm; subst.
+  eauto.
+  (* eapply H1.
+  apply H6.
+  eapply H2.
+  apply H3.
+  apply Hpst. *)
+Qed.
+
+Example hoare_asgn_example3 : forall (a:aexp) (n:nat),
+    {{a = n}}
+  X := a;
+  skip
+    {{X = n}}.
+Proof.
+  intros a n. 
+  eapply hoare_seq.
+  - (* right part of seq *)
+    apply hoare_skip.
+  - (* left part of seq *)
+    eapply hoare_consequence_pre.
+    + apply hoare_asgn.
+    + assn_auto.
+Qed.
+
+Example tst_seq_1 : 
+    {{ True }}
+  X := 1;
+  Y := 2
+    {{X = 1 /\ Y = 2}}.
+Proof.
+  eapply hoare_seq with (Q := assert (X = 1)).
+  - eapply hoare_consequence_pre with (P' := assert (X = 1 /\ Y = 2) [Y |-> 2]).
+    + apply hoare_asgn.
+    + assn_auto.
+  - apply hoare_consequence_pre with (P' := (X = 1) [X |-> 1]).
+    + apply hoare_asgn.
+    + assn_auto.
+Qed.
+
+
+Definition swap_program : com :=
+  <{ Z := X; X := Y; Y := Z }>.
+
+Theorem swap_exercise :
+  {{X <= Y}}
+  swap_program
+  {{Y <= X}}.
+Proof.
+  eapply hoare_seq with (Q := assert (Z <= Y)).
+  - eapply hoare_seq with (Q := assert (Z <= X)).
+    + apply hoare_consequence_pre with (P' := (Y <= X) [Y |-> Z]).
+      * apply hoare_asgn.
+      * assn_auto.
+    + apply hoare_consequence_pre with (P' := (Z <= X) [X |-> Y]).
+      * apply hoare_asgn.
+      * assn_auto.
+  - apply hoare_consequence_pre with (P' := (Z <= Y) [Z |-> X]).
+    * apply hoare_asgn.
+    * assn_auto.
+Qed.
+
+
+Theorem invalid_triple : ~ forall (a : aexp) (n : nat),
+    {{ a = n }}
+      X := 3; Y := a
+    {{ Y = n }}.
+Proof.
+  unfold hoare_triple.
+  intros H.
+  specialize H with (a := X) (n := 0).
+  simpl in *.
+  assert (G: (X !-> 0) =[ X := 3; Y := X ]=> (Y !-> 3; X !-> 3; X !-> 0)). {
+    eapply (E_Seq).
+    apply E_Asgn.
+    - simpl. reflexivity.
+    - eapply E_Asgn.
+      simpl. reflexivity.
+  }
+  assert (G': 3 = 0). {
+    apply (H _ _ G).
+    reflexivity.
+  }
+  discriminate G'.
+Qed.
+
+
+
+Definition bassn b : Assertion := fun st => (beval st b = true).
+Coercion bassn : bexp >-> Assertion.
+Arguments bassn /.
+
+Lemma bexp_eval_false : forall b st,
+  beval st b = false -> ~((bassn b) st).
+Proof. intros b st H. unfold not, bassn. intro H'. 
+  congruence. (* H and H' *) Qed.
+
+Hint Resolve bexp_eval_false : core.
+
+
+Theorem hoare_if : forall P Q (b:bexp) c1 c2,
+  {{ P /\ b }} c1 {{Q}} ->
+  {{ P /\ ~b}} c2 {{Q}} ->
+  {{P}} if b then c1 else c2 end {{Q}}.
+Proof. intros P Q b c1 c2. unfold hoare_triple.
+  intros H1 H2 st st' Hif Hpst.
+  inversion Hif; subst.
+  - (* if true *)
+    apply (H1 st st' H7). split; assumption.
+  - (* if false *)
+    apply (H2 st st' H7). split.
+    + apply Hpst.
+    + unfold not. simpl. intro Hcontra. congruence.
+Qed.
+
+Example if_example :
+    {{True}}
+  if (X = 0)
+    then Y := 2
+    else Y := X + 1
+  end
+    {{X <= Y}}.
+Proof.
+  apply hoare_if.
+  - (* Then *)
+    eapply hoare_consequence_pre.
+    + apply hoare_asgn.
+    + assn_auto. (* no progress *)
+      unfold "->>", assn_sub, t_update, bassn.
+      simpl. intros st [_ H].
+      apply eqb_eq in H.
+      rewrite H. lia.
+  - (* Else *)
+    eapply hoare_consequence_pre.
+    + apply hoare_asgn.
+    + assn_auto.
+Qed.
+
+Ltac assn_auto' :=
+  unfold "->>", assn_sub, t_update, bassn;
+  intros; simpl in *;
+  try rewrite -> eqb_eq in *; (* for equalities *)
+  auto; try lia.
+
+Example if_example''' :
+  {{True}}
+  if X = 0
+    then Y := 2
+    else Y := X + 1
+  end
+  {{X <= Y}}.
+Proof.
+  apply hoare_if; eapply hoare_consequence_pre;
+    try apply hoare_asgn; try assn_auto'.
+Qed.
+
+
+Ltac assn_auto'' :=
+  unfold "->>", assn_sub, t_update, bassn;
+  intros; simpl in *;
+  try rewrite -> eqb_eq in *;
+  try rewrite -> leb_le in *; (* for inequalities *)
+  auto; try lia.
+
+Theorem if_minus_plus :
+  {{True}}
+  if (X <= Y)
+    then Z := Y - X
+    else Y := X + Z
+  end
+  {{Y = X + Z}}.
+Proof.
+  apply hoare_if.
+  - eapply hoare_consequence_pre.
+    + apply hoare_asgn.
+    + assn_auto''.
+  - eapply hoare_consequence_pre.
+    + apply hoare_asgn.
+    + assn_auto''.
+Qed.
+
+
+
+
+
+
+
+
