softwarefoundations/vol2_plf/If1.v
@@ -1,0 +1,145 @@
+Set Warnings "-notation-overridden,-parsing,-deprecated-hint-without-locality".
+From PLF Require Import Maps.
+From Coq Require Import Bool.Bool.
+From Coq Require Import Arith.Arith.
+From Coq Require Import Arith.EqNat.
+From Coq Require Import Arith.PeanoNat. Import Nat.
+From Coq Require Import Lia.
+From PLF Require Import Imp.
+From PLF Require Import Hoare.
+
+From Coq Require Import Logic.FunctionalExtensionality.
+
+Module If1.
+
+Inductive com : Type :=
+  | CSkip : com
+  | CAsgn : string -> aexp -> com
+  | CSeq : com -> com -> com
+  | CIf : bexp -> com -> com -> com
+  | CWhile : bexp -> com -> com
+  | CIf1 : bexp -> com -> com.
+
+Notation "'if1' x 'then' y 'end'" :=
+         (CIf1 x y)
+         (in custom com at level 0, x custom com at level 99).
+Notation "'skip'" :=
+         CSkip 
+         (in custom com at level 0).
+Notation "x := y" :=
+         (CAsgn x y)
+         (in custom com at level 0, x constr at level 0, y at level 85, no associativity).
+Notation "x ; y" :=
+         (CSeq x y)
+         (in custom com at level 90, right associativity).
+Notation "'if' x 'then' y 'else' z 'end'" :=
+         (CIf x y z)
+         (in custom com at level 89, x at level 99, y at level 99, z at level 99).
+Notation "'while' x 'do' y 'end'" :=
+         (CWhile x y)
+         (in custom com at level 89, x at level 99, y at level 99).
+
+Reserved Notation "st '=[' c ']=>' st'"
+         (at level 40, c custom com at level 99, st constr, st' constr at next level).
+Inductive ceval : com -> state -> state -> Prop :=
+  | E_Skip : forall st,
+      st =[ skip ]=> st
+  | E_Asgn : forall st a1 n x,
+      aeval st a1 = n ->
+      st =[ x := a1 ]=> (x !-> n ; st)
+  | E_Seq : forall c1 c2 st st' st'',
+      st =[ c1 ]=> st' ->
+      st' =[ c2 ]=> st'' ->
+      st =[ c1 ; c2 ]=> st''
+  | E_IfTrue : forall st st' b c1 c2,
+      beval st b = true ->
+      st =[ c1 ]=> st' ->
+      st =[ if b then c1 else c2 end ]=> st'
+  | E_IfFalse : forall st st' b c1 c2,
+      beval st b = false ->
+      st =[ c2 ]=> st' ->
+      st =[ if b then c1 else c2 end ]=> st'
+  | E_WhileFalse : forall b st c,
+      beval st b = false ->
+      st =[ while b do c end ]=> st
+  | E_WhileTrue : forall st st' st'' b c,
+      beval st b = true ->
+      st =[ c ]=> st' ->
+      st' =[ while b do c end ]=> st'' ->
+      st =[ while b do c end ]=> st''
+  | E_If1True : forall st st' b c,
+      beval st b = true ->
+      st =[ c ]=> st' ->
+      st =[ if1 b then c end ]=> st'
+  | E_If1False : forall st b c,
+      beval st b = false ->
+      st =[ if1 b then c end ]=> st
+  where "st =[ c ]=> st'" := (ceval c st st').
+
+Hint Constructors ceval : core.
+
+Example if1true_test : empty_st =[ if1 X = 0 then X := 1 end ]=> (X !-> 1).
+Proof. eauto. Qed.
+
+Example if1false_test : (X !-> 2) =[ if1 X = 0 then X := 1 end ]=> (X !-> 2).
+Proof. eauto. Qed.
+
+Definition hoare_triple (P : Assertion) (c : com) (Q : Assertion) : Prop :=
+  forall st st', st =[ c ]=> st' -> P st -> Q st'.
+Hint Unfold hoare_triple : core.
+
+Notation "{{ P }} c {{ Q }}" := (hoare_triple P c Q)
+                                (at level 90, c custom com at level 99)
+                                : hoare_spec_scope.
+
+Theorem hoare_if1: forall P Q (b:bexp) c,
+  {{ P /\ b }} c {{Q}} ->
+  (P /\ ~b)%assertion ->> Q ->
+  {{P}} if1 b then c end {{Q}}.
+Proof. unfold hoare_triple. intros P Q b c H1 H2 st st' Hcom Hpst.
+  inversion Hcom; subst.
+  - apply (H1 st st' H6); simpl; split; assumption.
+  - apply H2; simpl; split.
+    + assumption.
+    + unfold not. intros Hcontra. congruence.
+Qed.
+
+Theorem hoare_consequence_pre : forall (P P' Q : Assertion) c,
+  {{P'}} c {{Q}} ->
+  P ->> P' ->
+  {{P}} c {{Q}}.
+Proof.
+  eauto.
+Qed.
+Theorem hoare_asgn : forall Q X a,
+  {{Q [X |-> a]}} (X := a) {{Q}}.
+Proof.
+  intros Q X a st st' Heval HQ.
+  inversion Heval; subst.
+  auto.
+Qed.
+
+Search (negb ?x <> true).
+Search ((?x =? ?m) = true -> ?x = ?m).
+
+Example hoare_if1_good: 
+  {{ X + Y = Z }}
+  if1 ~(Y = 0) then
+    X := X + Y
+  end
+  {{ X = Z }}.
+Proof.
+  apply hoare_if1; simpl.
+  - eapply hoare_consequence_pre.
+    apply hoare_asgn.
+    unfold "->>", assn_sub, t_update.
+    intros st [H _].
+    simpl. assumption.
+  - unfold "->>", assn_sub, t_update.
+    intros st [H Hy].
+    apply eq_true_negb_classical in Hy.
+    apply beq_nat_true in Hy.
+    lia.
+Qed.
+
+End If1.
